Flapjack/Test/StackRemove.lean
@@ -3,7 +3,8 @@ import Flapjack.StackRemove
 namespace Flapjack
 
 def stackRemoveTestConfig : StackRemoveConfig :=
-  { storeBase := 10, currHeap := 12, scratch := 31, addressScratch := 29 }
+  { storeBase := 10, currHeap := 12, scratch := 31, addressScratch := 29,
+    stackPointer := 20, bytesInWord := 8 }
 
 example :
     stackRemove stackRemoveTestConfig (.get 4 .heapLength : StackProg Nat) =
@@ -22,6 +23,55 @@ example :
       (.set .globals 6 : StackProg Nat) = _
   simp [stackRemoveFuel, stackRemoveSet, stackRemoveJoin,
     stackRemoveAddress, stackStorePosition, stackRemoveTestConfig]
+
+example :
+    stackRemove stackRemoveTestConfig (.stackAlloc 2 : StackProg Nat) =
+      .seq (.const 31 16) (.arith .sub 20 20 31) := by
+  simp [stackRemove, stackRemoveFuel, stackRemoveStackAlloc,
+    stackRemoveStackDelta, stackRemoveJoin, stackRemoveTestConfig]
+
+example :
+    stackRemove stackRemoveTestConfig (.stackFree 2 : StackProg Nat) =
+      .seq (.const 31 16) (.arith .add 20 20 31) := by
+  simp [stackRemove, stackRemoveFuel, stackRemoveStackFree,
+    stackRemoveStackDelta, stackRemoveJoin, stackRemoveTestConfig]
+
+example :
+    stackRemove stackRemoveTestConfig (.stackAlloc 256 : StackProg Nat) =
+      .seq
+        (.seq (.const 31 2040) (.arith .sub 20 20 31))
+        (.seq (.const 31 8) (.arith .sub 20 20 31)) := by
+  simp [stackRemove, stackRemoveFuel, stackRemoveStackAlloc,
+    stackRemoveStackDelta, stackRemoveJoin, stackRemoveTestConfig]
+
+example :
+    stackRemove stackRemoveTestConfig (.stackStore 6 2 : StackProg Nat) =
+      .seq (.arith .or 31 6 6)
+        (.seq (.seq (.const 29 16) (.arith .add 29 20 29))
+          (.inst (.mem .store 31 29))) := by
+  simp [stackRemove, stackRemoveFuel, stackRemoveStackStore,
+    stackRemoveStackAddress, stackRemoveMove, stackRemoveJoin,
+    stackRemoveTestConfig]
+
+example :
+    stackRemove stackRemoveTestConfig (.stackLoad 6 2 : StackProg Nat) =
+      .seq (.seq (.const 29 16) (.arith .add 29 20 29))
+        (.inst (.mem .load 6 29)) := by
+  simp [stackRemove, stackRemoveFuel, stackRemoveStackLoad,
+    stackRemoveStackAddress, stackRemoveJoin, stackRemoveTestConfig]
+
+example :
+    stackRemove stackRemoveTestConfig (.stackLoadAny 6 7 : StackProg Nat) =
+      .seq (.arith .add 29 20 7) (.inst (.mem .load 6 29)) := by
+  simp [stackRemove, stackRemoveFuel, stackRemoveStackLoadAny,
+    stackRemoveJoin, stackRemoveTestConfig]
+
+example :
+    stackRemove stackRemoveTestConfig (.stackStoreAny 6 7 : StackProg Nat) =
+      .seq (.arith .or 31 6 6)
+        (.seq (.arith .add 29 20 7) (.inst (.mem .store 31 29))) := by
+  simp [stackRemove, stackRemoveFuel, stackRemoveStackStoreAny,
+    stackRemoveMove, stackRemoveJoin, stackRemoveTestConfig]
 
 example :
     stackRemove stackRemoveTestConfig (.get 4 .currHeap : StackProg Nat) =
